pop for aux tapes.

Cslib/Computability/Machines/MultiTapeTuring/PopRoutine.lean
@@ -12,6 +12,7 @@ import Cslib.Foundations.Data.RelatesInSteps
 public import Cslib.Computability.Machines.MultiTapeTuring.Basic
 public import Cslib.Computability.Machines.MultiTapeTuring.ListEncoding
 public import Cslib.Computability.Machines.MultiTapeTuring.WithTapes
+public import Cslib.Computability.Machines.MultiTapeTuring.TMWithAuxTapes
 
 -- TODO create a "common file"
 import Cslib.Computability.Machines.SingleTapeTuring.Basic
@@ -40,6 +41,20 @@ public theorem pop_eval_list {k : ℕ} {i : Fin k.succ}
   {tapes : Fin k.succ → List (List α)}
   {h_not_empty : tapes i ≠ []} :
   (pop i).eval_list tapes = .some (Function.update tapes i (tapes i).tail) := by
+  sorry
+
+public def pop' {k aux : ℕ} (i : ℕ) (h_i_lt : i < k := by decide) :
+    MultiTapeTMWithAuxTapes k aux (WithSep α) :=
+  (pop₁.allocate_aux_tapes aux).with_tapes #v[⟨i, h_i_lt⟩]
+    (h_le_k := by omega)
+    (h_le_aux := by rfl)
+
+@[simp, grind =]
+public theorem pop'_eval_list {k aux i : ℕ} {h_i_lt : i < k}
+  {tapes : Fin k → List (List α)}
+  {h_not_empty : tapes ⟨i, h_i_lt⟩ ≠ []} :
+  (pop' (aux := aux) i h_i_lt).eval_list tapes = .some
+    (Function.update tapes ⟨i, h_i_lt⟩ (tapes ⟨i, h_i_lt⟩).tail) := by
   sorry
 
 end Routines
